src/Kleene_Post.lean
@@ -1,4 +1,4 @@
-import reducibility computable_function fis
+import reducibility function fis
 
 open encodable denumerable roption
 
@@ -10,35 +10,35 @@ lemma bnot_ne (b) : b ≠ !b := by cases b; simp
 open primrec
 
 theorem extendable_suffix {l₀ n e} {A : ℕ → bool}
-  (h : ∀ l : list bool, ¬(⟦e⟧ᵪ^(l ++ l₀).rnth n).dom) (hl₀ : l₀.rnth ⊆* (λ x, A x)) :
-  ¬(⟦e⟧ᵪ^(λ x, some (A x)) n).dom := λ C,
+  (h : ∀ l : list bool, ¬(⟦e⟧ᵪ*(l ++ l₀).rnth n).dom) (hl₀ : l₀.rnth ⊆* ↑ₒA) :
+  ¬(⟦e⟧ᵪ^A n).dom := λ C,
 begin
   rcases roption.dom_iff_mem.mp C with ⟨b, hb⟩,
   rcases rpartrec.eval_inclusion hb with ⟨s, hs⟩,
   have := initial_subseq hl₀ s, rcases this with ⟨l, hl⟩,
-  suffices : b ∈ (⟦e⟧ᵪ^((l ++ l₀).rnth) n),
+  suffices : b ∈ (⟦e⟧ᵪ*((l ++ l₀).rnth) n),
   { rcases this with ⟨lmm, _⟩, exact h _ lmm },
   apply hs, simp, intros m c em hc,
   have : (initial_code (λ (x : ℕ), A x) s).rnth m = c, simp[em, hc],
   exact hl _ _ this
 end
 
-def O₀ := {x : ℕ × list bool × ℕ | ∃ l, (⟦x.1⟧ᵪ^(l ++ x.2.1).rnth x.2.2).dom}
+def O₀ := {x : ℕ × list bool × ℕ | ∃ l, (⟦x.1⟧ᵪ*(l ++ x.2.1).rnth x.2.2).dom}
 
-def O₁ := {x : ℕ × list bool × ℕ | (⟦x.1⟧ᵪ^x.2.1.rnth x.2.2).dom}
+def O₁ := {x : ℕ × list bool × ℕ | (⟦x.1⟧ᵪ*x.2.1.rnth x.2.2).dom}
 
 theorem O₀_0'computable : O₀ ≤ₜ ∅′ :=
 begin
-  let f := (λ (x : ℕ × list bool × ℕ) l, ⟦x.1⟧ᵪ^(l ++ x.2.1).rnth x.2.2),
+  let f := (λ (x : ℕ × list bool × ℕ) l, ⟦x.1⟧ᵪ*(l ++ x.2.1).rnth x.2.2),
   have := (fst.comp fst).pair ((list_append.comp snd (fst.comp $ snd.comp fst)).pair
     (snd.comp $ snd.comp fst)),
-  have : partrec₂ f := (partrec.eval_list_partrec ℕ bool).comp this.to_comp,
+  have : partrec₂ f := (partrec.eval_list ℕ bool).comp this.to_comp,
   have := domex_0'computable this,
   exact this
 end
 
 theorem O₁_0'computable : O₁ ≤ₜ ∅′ :=
-dom_0'computable (partrec.eval_list_partrec ℕ bool)
+dom_0'computable (partrec.eval_list ℕ bool)
 
 namespace Kleene_Post
 
@@ -49,23 +49,23 @@ noncomputable def L : ℕ →. list bool × list bool
   match s.bodd with
   | ff := do σ ← L s,
     if (e, σ.2, σ.1.length) ∈ O₀
-    then do l ← epsilon (chr $ λ l, (⟦e⟧ᵪ^(l ++ σ.2).rnth σ.1.length).dom),
-            b ← (⟦e⟧ᵪ^((l ++ σ.2).rnth) σ.1.length),
+    then do l ← epsilon (chr $ λ l, (⟦e⟧ᵪ*(l ++ σ.2).rnth σ.1.length).dom),
+            b ← (⟦e⟧ᵪ*(l ++ σ.2).rnth σ.1.length),
             some (!b :: σ.1, l ++ σ.2)
     else some (ff :: σ.1, σ.2)
   | tt := do σ ← L s,
     if (e, σ.1, σ.2.length) ∈ O₀
-    then do l ← epsilon (chr $ λ l, (⟦e⟧ᵪ^((l ++ σ.1).rnth) σ.2.length).dom),
-            b ← (⟦e⟧ᵪ^((l ++ σ.1).rnth) σ.2.length),
+    then do l ← epsilon (chr $ λ l, (⟦e⟧ᵪ*(l ++ σ.1).rnth σ.2.length).dom),
+            b ← (⟦e⟧ᵪ*(l ++ σ.1).rnth σ.2.length),
             some (l ++ σ.1, !b :: σ.2)
     else some (σ.1, ff :: σ.2)
   end
 
 lemma fffL_0'partrec'₀ :
   (λ (a : ℕ × list bool × list bool),
-    epsilon (chr (λ l, (⟦a.fst.div2⟧ᵪ^((l ++ a.snd.fst).rnth) a.snd.snd.length).dom)) >>=
-    λ l, (⟦a.1.div2⟧ᵪ^((l ++ a.2.1).rnth) a.2.2.length >>=
-    λ b, some (l ++ a.2.1, !b :: a.2.2))) partrec_in chr. O₁ :=
+    epsilon (chr (λ l, (⟦a.fst.div2⟧ᵪ*(l ++ a.snd.fst).rnth a.snd.snd.length).dom)) >>=
+    λ l, (⟦a.1.div2⟧ᵪ*(l ++ a.2.1).rnth a.2.2.length >>=
+    λ b, some (l ++ a.2.1, !b :: a.2.2))) partrec_in! chr O₁ :=
 begin
   simp [(>>=)],
   apply rpartrec.bind',
@@ -73,7 +73,7 @@ begin
     let p := (λ x : (ℕ × list bool × list bool) × list bool,
       chr O₁ (x.1.1.div2, x.2 ++ x.1.2.1, x.1.2.2.length)),
     have : ∀ a : ℕ × list bool × list bool,
-      chr (λ l, (⟦a.1.div2⟧ᵪ^((l ++ a.2.1).rnth) a.2.2.length).dom) = λ l, p (a, l),
+      chr (λ l, (⟦a.1.div2⟧ᵪ*(l ++ a.2.1).rnth a.2.2.length).dom) = λ l, p (a, l),
     { intros a, funext x, apply chr_ext.mpr, simp [O₁] }, simp [this],
     have := (nat_div2.comp $ fst.comp fst).pair 
       ((list_append.comp snd (fst.comp $ snd.comp fst)).pair 
@@ -87,23 +87,23 @@ end
 
 lemma L_0'partrec'₀ :
   (λ (a : ℕ × list bool × list bool),
-    epsilon (chr (λ l, (⟦a.fst.div2⟧ᵪ^((l ++ a.snd.fst).rnth) a.snd.snd.length).dom)) >>=
-    λ l, (⟦a.1.div2⟧ᵪ^((l ++ a.2.1).rnth) a.2.2.length >>=
-    λ b, some (l ++ a.2.1, !b :: a.2.2))) partrec_in chr. ∅′ :=
+    epsilon (chr (λ l, (⟦a.fst.div2⟧ᵪ*(l ++ a.snd.fst).rnth a.snd.snd.length).dom)) >>=
+    λ l, (⟦a.1.div2⟧ᵪ*(l ++ a.2.1).rnth a.2.2.length >>=
+    λ b, some (l ++ a.2.1, !b :: a.2.2))) partrec_in! chr ∅′ :=
 begin
   let p := (λ x : (ℕ × list bool × list bool) × list bool,
     chr O₁ (x.1.1.div2, x.2 ++ x.1.2.1, x.1.2.2.length)),
   have : ∀ a : ℕ × list bool × list bool,
-    chr (λ l, (⟦a.1.div2⟧ᵪ^((l ++ a.2.1).rnth) a.2.2.length).dom) = λ l, p (a, l),
+    chr (λ l, (⟦a.1.div2⟧ᵪ*(l ++ a.2.1).rnth a.2.2.length).dom) = λ l, p (a, l),
   { intros a, funext x, apply chr_ext.mpr, simp [O₁] }, simp [this],
-  have lmm : (λ a, epsilon (λ x, p (a, x))) partrec_in chr. ∅′,
+  have lmm : (λ a, epsilon (λ x, p (a, x))) partrec_in! chr ∅′,
   { have := (nat_div2.comp $ fst.comp fst).pair 
       ((list_append.comp snd (fst.comp $ snd.comp fst)).pair 
       (list_length.comp $ snd.comp $ snd.comp fst)),
     have := (classical_iff.mp O₁_0'computable).comp this.to_comp.to_rcomp,
     exact (rpartrec.epsilon_rpartrec p).trans this },
   let g := λ x : (ℕ × list bool × list bool) × list bool,
-    (⟦x.1.1.div2⟧ᵪ^((x.2 ++ x.1.2.1).rnth) x.1.2.2.length).bind
+    (⟦x.1.1.div2⟧ᵪ*(x.2 ++ x.1.2.1).rnth x.1.2.2.length).bind
     (λ b, some (x.2 ++ x.1.2.1, !b :: x.1.2.2)),
   have lmm1 : partrec g,
   { let m := (λ x : (ℕ × list bool × list bool) × list bool,
@@ -111,7 +111,7 @@ begin
     have pm : primrec m := (nat_div2.comp $ fst.comp fst).pair
       ((list_append.comp snd (fst.comp $ snd.comp fst)).pair
       (list_length.comp $ snd.comp $ snd.comp fst)),
-    have lmm1 := (partrec.eval_list_partrec ℕ bool).comp pm.to_comp, simp [m] at lmm1,
+    have lmm1 := (partrec.eval_list ℕ bool).comp pm.to_comp, simp [m] at lmm1,
     let h := (λ (x : (ℕ × list bool × list bool) × list bool) (b : bool),
       (x.2 ++ x.1.2.1, !b :: x.1.2.2)),
     have ph : primrec₂ h := (list_append.comp (snd.comp fst) 
@@ -124,23 +124,23 @@ end
 
 lemma L_0'partrec'₁ :
   (λ (a : ℕ × list bool × list bool),
-    epsilon (chr (λ l, (⟦a.fst.div2⟧ᵪ^((l ++ a.snd.snd).rnth) a.snd.fst.length).dom)) >>=
-    λ l, ⟦a.1.div2⟧ᵪ^((l ++ a.2.2).rnth) a.2.1.length >>=
-    λ b, some (!b :: a.2.1, l ++ a.2.2)) partrec_in chr. ∅′ :=
+    epsilon (chr (λ l, (⟦a.fst.div2⟧ᵪ*(l ++ a.snd.snd).rnth a.snd.fst.length).dom)) >>=
+    λ l, ⟦a.1.div2⟧ᵪ*(l ++ a.2.2).rnth a.2.1.length >>=
+    λ b, some (!b :: a.2.1, l ++ a.2.2)) partrec_in! chr ∅′ :=
 begin
   let p := (λ x : (ℕ × list bool × list bool) × list bool,
     chr O₁ (x.1.1.div2, x.2 ++ x.1.2.2, x.1.2.1.length)),
   have : ∀ a : ℕ × list bool × list bool,
-    chr (λ l, (⟦a.1.div2⟧ᵪ^((l ++ a.2.2).rnth) a.2.1.length).dom) = λ l, p (a, l),
+    chr (λ l, (⟦a.1.div2⟧ᵪ*(l ++ a.2.2).rnth a.2.1.length).dom) = λ l, p (a, l),
   { intros a, funext x, apply chr_ext.mpr, simp [O₁] },
-  have lmm : (λ a, epsilon (λ x, p (a, x))) partrec_in chr. ∅′,
+  have lmm : (λ a, epsilon (λ x, p (a, x))) partrec_in! chr ∅′,
   { have := (nat_div2.comp $ fst.comp fst).pair 
       ((list_append.comp snd (snd.comp $ snd.comp fst)).pair 
       (list_length.comp $ fst.comp $ snd.comp fst)),
     have := (classical_iff.mp O₁_0'computable).comp this.to_comp.to_rcomp,
     exact (rpartrec.epsilon_rpartrec p).trans this },
   let g := λ x : (ℕ × list bool × list bool) × list bool,
-    (⟦x.1.1.div2⟧ᵪ^((x.2 ++ x.1.2.2).rnth) x.1.2.1.length).bind
+    (⟦x.1.1.div2⟧ᵪ*(x.2 ++ x.1.2.2).rnth x.1.2.1.length).bind
     (λ b, some (!b :: x.1.2.1, x.2 ++ x.1.2.2)),
   have lmm1 : partrec g,
   { let m := (λ x : (ℕ × list bool × list bool) × list bool,
@@ -148,7 +148,7 @@ begin
     have pm : primrec m := (nat_div2.comp $ fst.comp fst).pair
       ((list_append.comp snd (snd.comp $ snd.comp fst)).pair
       (list_length.comp $ fst.comp $ snd.comp fst)),
-    have lmm1 := (partrec.eval_list_partrec ℕ bool).comp pm.to_comp, simp [m] at lmm1,
+    have lmm1 := (partrec.eval_list ℕ bool).comp pm.to_comp, simp [m] at lmm1,
     let h := (λ (x : (ℕ × list bool × list bool) × list bool) (b : bool),
       (!b :: x.1.2.1, x.2 ++ x.1.2.2)),
     have ph : primrec₂ h := 
@@ -159,7 +159,7 @@ begin
   exact this
 end
 
-lemma L_0'partrec : L partrec_in (chr. ∅′) :=
+lemma L_0'partrec : L partrec_in! chr ∅′ :=
 begin
   let h : ℕ × ℕ × (list bool × list bool) →. list bool × list bool := λ x,
     let s := x.2.1,
@@ -167,16 +167,16 @@ begin
         e := s.div2 in
     cond s.bodd
       (cond (chr O₀ (e, σ.1, σ.2.length))
-        (do l ← epsilon (chr $ λ l, (⟦e⟧ᵪ^((l ++ σ.1).rnth) σ.2.length).dom),
-            b ← (⟦e⟧ᵪ^((l ++ σ.1).rnth) σ.2.length),
+        (do l ← epsilon (chr $ λ l, (⟦e⟧ᵪ*(l ++ σ.1).rnth σ.2.length).dom),
+            b ← (⟦e⟧ᵪ*(l ++ σ.1).rnth σ.2.length),
             some (l ++ σ.1, !b :: σ.2))
         (some (σ.1, ff :: σ.2)))    
       (cond (chr O₀ (e, σ.2, σ.1.length))
-        (do l ← epsilon (chr $ λ l, (⟦e⟧ᵪ^((l ++ σ.2).rnth) σ.1.length).dom),
-            b ← (⟦e⟧ᵪ^((l ++ σ.2).rnth) σ.1.length),
+        (do l ← epsilon (chr $ λ l, (⟦e⟧ᵪ*(l ++ σ.2).rnth σ.1.length).dom),
+            b ← (⟦e⟧ᵪ*(l ++ σ.2).rnth σ.1.length),
             some (!b :: σ.1, l ++ σ.2))
         (some (ff :: σ.1, σ.2))),
-  have : h partrec_in (chr. ∅′),
+  have : h partrec_in! chr ∅′,
   { simp [h], apply rpartrec.cond,
     { exact (primrec.nat_bodd.comp $ primrec.fst.comp primrec.snd).to_comp.to_rcomp },
     { apply rpartrec.cond,
@@ -203,7 +203,7 @@ begin
     (rcomputable.const (([], []) : list bool × list bool)) this,
   exact (this.of_eq $ λ s, by 
   { simp, induction s with s0 ih; simp [L],
-    cases C : s0.bodd; simp [C, L, h] at ih ⊢; rw ih; congr; funext; simp [C, O₀, cond_if_eq] })
+    cases C : s0.bodd; simp [C, L, h] at ih ⊢; rw ih; congr; funext; simp [C, O₀, cond_if_eq], }),
 end
 
 lemma I_defined : ∀ s, (L s).dom 
@@ -216,7 +216,7 @@ lemma I_defined : ∀ s, (L s).dom
       { refine ⟨IH, _⟩,
         by_cases C : (s.div2, ((L s).get IH).snd, ((L s).get IH).fst.length) ∈ O₀;
         simp [C], simp [O₀, set.set_of_app_iff] at C, refine ⟨C, _⟩,
-        have : ∃ l, l ∈ epsilon (chr $ λ l, (⟦s.div2⟧ᵪ^((l ++ ((L s).get IH).2).rnth) ((L s).get IH).1.length).dom),
+        have : ∃ l, l ∈ epsilon (chr $ λ l, (⟦s.div2⟧ᵪ*(l ++ ((L s).get IH).2).rnth ((L s).get IH).1.length).dom),
         { simp[←roption.dom_iff_mem], exact C },
         rcases this with ⟨l, hl⟩,
         have hb := epsilon_witness hl, simp only [chr_iff, roption.dom_iff_mem] at hb,
@@ -225,7 +225,7 @@ lemma I_defined : ∀ s, (L s).dom
       { refine ⟨IH, _⟩,
         by_cases C : (s.div2, ((L s).get IH).1, ((L s).get IH).2.length) ∈ O₀;
         simp [C], simp [O₀, set.set_of_app_iff] at C, refine ⟨C, _⟩,
-        have : ∃ l, l ∈ epsilon (chr $ λ l, (⟦s.div2⟧ᵪ^((l ++ ((L s).get IH).1).rnth) ((L s).get IH).2.length).dom),
+        have : ∃ l, l ∈ epsilon (chr $ λ l, (⟦s.div2⟧ᵪ*(l ++ ((L s).get IH).1).rnth ((L s).get IH).2.length).dom),
         { simp[←roption.dom_iff_mem], exact C },
         rcases this with ⟨l, hl⟩,
         have hb := epsilon_witness hl, simp only [chr_iff, roption.dom_iff_mem] at hb,
@@ -241,17 +241,17 @@ def I₀ : set ℕ := limit L₀
 
 def I₁ : set ℕ := limit L₁
 
-lemma L₀_0'computable : L₀ computable_in chr. ∅′ :=
+lemma L₀_0'computable : L₀ computable_in! chr ∅′ :=
 begin
   have := (rcomputable.total_computable I_defined),
-  have : (λ (a : ℕ), (L a).get _) computable_in chr. ∅′ := rpartrec.trans this L_0'partrec,
+  have : (λ (a : ℕ), (L a).get _) computable_in! chr ∅′ := rpartrec.trans this L_0'partrec,
   exact rcomputable.fst.comp this,
 end
 
-lemma L₁_0'computable : L₁ computable_in chr. ∅′ :=
+lemma L₁_0'computable : L₁ computable_in! chr ∅′ :=
 begin
   have := (rcomputable.total_computable I_defined),
-  have : (λ (a : ℕ), (L a).get _) computable_in chr. ∅′ := rpartrec.trans this L_0'partrec,
+  have : (λ (a : ℕ), (L a).get _) computable_in! chr ∅′ := rpartrec.trans this L_0'partrec,
   exact rcomputable.snd.comp this,
 end
 
@@ -260,7 +260,7 @@ lemma L₀_length (e) :
 begin
   simp[fis, L₀, L], simp [L, show ∀ s, L s = some (L₀ s, L₁ s), by simp[L₀, L₁]],
   { by_cases C : (e, L₁ (bit0 e), (L₀ (bit0 e)).length) ∈ O₀; simp [C],
-    have : ∃ l, l ∈ epsilon (chr $ λ l, (⟦e⟧ᵪ^((l ++ L₁ (bit0 e)).rnth) (L₀ (bit0 e)).length).dom),
+    have : ∃ l, l ∈ epsilon (chr $ λ l, (⟦e⟧ᵪ*(l ++ L₁ (bit0 e)).rnth (L₀ (bit0 e)).length).dom),
     { simp[←roption.dom_iff_mem], exact C },
     rcases this with ⟨l, hl⟩,
     have hb := epsilon_witness hl, simp only [chr_iff, roption.dom_iff_mem] at hb,
@@ -273,7 +273,7 @@ lemma L₁_length (e) :
 begin
   simp[fis, L₁, L], simp [L, show ∀ s, L s = some (L₀ s, L₁ s), by simp[L₀, L₁]],
   { by_cases C : (e, L₀ (bit1 e), (L₁ (bit1 e)).length) ∈ O₀; simp [C],
-    have : ∃ l, l ∈ epsilon (chr $ λ l, (⟦e⟧ᵪ^((l ++ L₀ (bit1 e)).rnth) (L₁ (bit1 e)).length).dom),
+    have : ∃ l, l ∈ epsilon (chr $ λ l, (⟦e⟧ᵪ*(l ++ L₀ (bit1 e)).rnth (L₁ (bit1 e)).length).dom),
     { simp[←roption.dom_iff_mem], exact C },
     rcases this with ⟨l, hl⟩,
     have hb := epsilon_witness hl, simp only [chr_iff, roption.dom_iff_mem] at hb,
@@ -287,14 +287,14 @@ begin
   let e := s.div2,
   simp[fis, L₀, L], cases M : s.bodd; simp [M, L, show L s = some (L₀ s, L₁ s), by simp[L₀, L₁]],
   { by_cases C : (s.div2, L₁ s, (L₀ s).length) ∈ O₀; simp [C],
-    have : ∃ l, l ∈ epsilon (chr $ λ l, (⟦s.div2⟧ᵪ^((l ++ L₁ s).rnth) (L₀ s).length).dom),
+    have : ∃ l, l ∈ epsilon (chr $ λ l, (⟦s.div2⟧ᵪ*(l ++ L₁ s).rnth (L₀ s).length).dom),
     { simp[←roption.dom_iff_mem], exact C },
     rcases this with ⟨l, hl⟩,
     have hb := epsilon_witness hl, simp only [chr_iff, roption.dom_iff_mem] at hb,
     rcases hb with ⟨b, hb⟩,
     simp [roption.eq_some_iff.mpr hl, roption.eq_some_iff.mpr hb] },  
   { by_cases C : (s.div2, L₀ s, (L₁ s).length) ∈ O₀; simp [C],
-    have : ∃ l, l ∈ epsilon (chr $ λ l, (⟦s.div2⟧ᵪ^((l ++ L₀ s).rnth) (L₁ s).length).dom),
+    have : ∃ l, l ∈ epsilon (chr $ λ l, (⟦s.div2⟧ᵪ*(l ++ L₀ s).rnth (L₁ s).length).dom),
     { simp[←roption.dom_iff_mem], exact C },
     rcases this with ⟨l, hl⟩,
     have hb := epsilon_witness hl, simp only [chr_iff, roption.dom_iff_mem] at hb,
@@ -308,14 +308,14 @@ begin
   let e := s.div2,
   simp[fis, L₁, L], cases M : s.bodd; simp [M, L, show L s = some (L₀ s, L₁ s), by simp[L₀, L₁]],
   { by_cases C : (s.div2, L₁ s, (L₀ s).length) ∈ O₀; simp [C],
-    have : ∃ l, l ∈ epsilon (chr $ λ l, (⟦s.div2⟧ᵪ^((l ++ L₁ s).rnth) (L₀ s).length).dom),
+    have : ∃ l, l ∈ epsilon (chr $ λ l, (⟦s.div2⟧ᵪ*(l ++ L₁ s).rnth (L₀ s).length).dom),
     { simp[←roption.dom_iff_mem], exact C },
     rcases this with ⟨l, hl⟩,
     have hb := epsilon_witness hl, simp only [chr_iff, roption.dom_iff_mem] at hb,
     rcases hb with ⟨b, hb⟩,
     simp [roption.eq_some_iff.mpr hl, roption.eq_some_iff.mpr hb] },  
   { by_cases C : (s.div2, L₀ s, (L₁ s).length) ∈ O₀; simp [C],
-    have : ∃ l, l ∈ epsilon (chr $ λ l, (⟦s.div2⟧ᵪ^((l ++ L₀ s).rnth) (L₁ s).length).dom),
+    have : ∃ l, l ∈ epsilon (chr $ λ l, (⟦s.div2⟧ᵪ*(l ++ L₀ s).rnth (L₁ s).length).dom),
     { simp[←roption.dom_iff_mem], exact C },
     rcases this with ⟨l, hl⟩,
     have hb := epsilon_witness hl, simp only [chr_iff, roption.dom_iff_mem] at hb,
@@ -356,15 +356,15 @@ lemma I₁_0'computable : I₁ ≤ₜ ∅′ :=
 classical_iff.mpr $ (L₁_fiss.limit_fullfiss_computable L₁_full).trans L₁_0'computable
 
 lemma requirement₀ (e) : ∃ w : ℕ,
-  !chr I₀ w ∈ ⟦e⟧ᵪ^(chr* I₁) w ∨ ¬(⟦e⟧ᵪ^(chr* I₁) w).dom :=
+  !chr I₀ w ∈ ⟦e⟧ᵪ^(chr I₁) w ∨ ¬(⟦e⟧ᵪ^(chr I₁) w).dom :=
 begin
   let i := 2*e,
   let w := (L₀ i).length,
   use w,
   by_cases C : (e, L₁ i, w) ∈ O₀,
   { left,
-    show !chr I₀ w ∈ ⟦e⟧ᵪ^(chr* I₁) w,
-    have : ∃ l, l ∈ epsilon (chr (λ l, (⟦e⟧ᵪ^((l ++ L₁ i).rnth) w).dom)),
+    show !chr I₀ w ∈ ⟦e⟧ᵪ^(chr I₁) w,
+    have : ∃ l, l ∈ epsilon (chr (λ l, (⟦e⟧ᵪ*((l ++ L₁ i).rnth) w).dom)),
     { simp[←roption.dom_iff_mem] at C ⊢, exact C },
     rcases this with ⟨l, hl⟩,
     have hb := epsilon_witness hl, simp only [chr_iff, roption.dom_iff_mem] at hb,
@@ -379,25 +379,25 @@ begin
       simp [nL₀, list.rnth] at this, apply this,
       rw (show w = (L₀ i).reverse.length, by simp),
       simp only [list.nth_concat_length] },
-    have lmm1 : b ∈ ⟦e⟧ᵪ^(chr* I₁) w,
+    have lmm1 : b ∈ ⟦e⟧ᵪ^(chr I₁) w,
     { rcases rpartrec.eval_inclusion hb with ⟨s, hs⟩, apply hs, simp,
       have := L₁_fiss.fiss_subseq_limit (i + 1), simp[nL₁, subseq] at this,
       exact (λ n c _, this n c) },
     simp[lmm, lmm1] },
   { right, simp [O₀] at C,
-    have : (L₁ i).rnth ⊆* chr* I₁, from L₁_fiss.fiss_subseq_limit _,
+    have : (L₁ i).rnth ⊆* ↑ₒ(chr I₁), from L₁_fiss.fiss_subseq_limit _,
     exact extendable_suffix C this }
 end
 
 lemma requirement₁ (e) : ∃ w : ℕ,
-  !chr I₁ w ∈ ⟦e⟧ᵪ^(chr* I₀) w ∨ ¬(⟦e⟧ᵪ^(chr* I₀) w).dom :=
+  !chr I₁ w ∈ ⟦e⟧ᵪ^(chr I₀) w ∨ ¬(⟦e⟧ᵪ^(chr I₀) w).dom :=
 begin
   let i := bit1 e,
   let w := (L₁ i).length,
   use w,
   by_cases C : (e, L₀ i, w) ∈ O₀,
-  { left, show !chr I₁ w ∈ ⟦e⟧ᵪ^(chr* I₀) w,
-    have : ∃ l, l ∈ epsilon (chr $ λ l, (⟦e⟧ᵪ^((l ++ L₀ i).rnth) w).dom),
+  { left, show !chr I₁ w ∈ ⟦e⟧ᵪ^(chr I₀) w,
+    have : ∃ l, l ∈ epsilon (chr $ λ l, (⟦e⟧ᵪ*(l ++ L₀ i).rnth w).dom),
     { simp[←roption.dom_iff_mem] at C ⊢, exact C },
     rcases this with ⟨l, hl⟩,
     have hb := epsilon_witness hl, simp only [chr_iff, roption.dom_iff_mem] at hb,
@@ -412,41 +412,41 @@ begin
       simp [nL₁, list.rnth] at this, apply this,
       rw (show w = (L₁ i).reverse.length, by simp),
       simp only [list.nth_concat_length] },
-    have lmm1 : b ∈ ⟦e⟧ᵪ^(chr* I₀) w,
+    have lmm1 : b ∈ ⟦e⟧ᵪ^(chr I₀) w,
     { rcases rpartrec.eval_inclusion hb with ⟨s, hs⟩, apply hs, simp,
       have := L₀_fiss.fiss_subseq_limit (i + 1), simp[nL₀, subseq] at this,
       exact (λ n c _, this n c) },
     simp[lmm, lmm1] },
   { right, simp [O₀] at C,
-    have : (L₀ i).rnth ⊆* chr* I₀, from L₀_fiss.fiss_subseq_limit _,
+    have : (L₀ i).rnth ⊆* ↑ₒ(chr I₀), from L₀_fiss.fiss_subseq_limit _,
     exact extendable_suffix C this }
 end
 
 lemma incomparable₀ : ¬I₀ ≤ₜ I₁ :=
 begin
   assume hyp : I₀ ≤ₜ I₁,
-  have : ∃ e, ⟦e⟧ᵪ^(chr* I₁) = chr I₀ :=
+  have : ∃ e, ⟦e⟧ᵪ^(chr I₁) = chr I₀ :=
     rpartrec.rpartrec_univ_iff_total.mp (classical_iff.mp hyp),
   rcases this with ⟨e, lmm_e⟩,
-  have lmm : ∀ n, (chr I₀ n) ∈ (⟦e⟧ᵪ^(chr* I₁) n), simp[lmm_e],
+  have lmm : ∀ n, (chr I₀ n) ∈ (⟦e⟧ᵪ^(chr I₁) n), simp[lmm_e],
   rcases requirement₀ e with ⟨w, lmm_w⟩, cases lmm_w,
   { have : chr I₀ w = !chr I₀ w := roption.mem_unique (lmm w) lmm_w,
     show false, from bnot_ne _ this },
-  { have : (⟦e⟧ᵪ^(chr* I₁) w).dom, { rcases lmm w with ⟨h, _⟩, exact h },
+  { have : (⟦e⟧ᵪ^(chr I₁) w).dom, { rcases lmm w with ⟨h, _⟩, exact h },
     contradiction }
 end
 
 lemma incomparable₁ : ¬I₁ ≤ₜ I₀ :=
 begin
   assume hyp : I₁ ≤ₜ I₀,
-  have : ∃ e, ⟦e⟧ᵪ^(chr* I₀) = chr I₁ :=
+  have : ∃ e, ⟦e⟧ᵪ^(chr I₀) = chr I₁ :=
     rpartrec.rpartrec_univ_iff_total.mp (classical_iff.mp hyp),
   rcases this with ⟨e, lmm_e⟩,
-  have lmm : ∀ n, (chr I₁ n) ∈ (⟦e⟧ᵪ^(chr* I₀) n), simp[lmm_e],
+  have lmm : ∀ n, (chr I₁ n) ∈ (⟦e⟧ᵪ^(chr I₀) n), simp[lmm_e],
   rcases requirement₁ e with ⟨w, lmm_w⟩, cases lmm_w,
   { have : chr I₁ w = !chr I₁ w := roption.mem_unique (lmm w) lmm_w,
     show false, from bnot_ne _ this },
-  { have : (⟦e⟧ᵪ^(chr* I₀) w).dom, { rcases lmm w with ⟨h, _⟩, exact h },
+  { have : (⟦e⟧ᵪ^(chr I₀) w).dom, { rcases lmm w with ⟨h, _⟩, exact h },
     contradiction }
 end
 
